Refactor Importable

io/Compile.IIO.To.ILang.fst
@@ -39,10 +39,10 @@ class importable (t : Type u#a) (pi:monitorable_prop) (rcs:tree pck_rc) (fl:eras
 
 (** *** Exportable instances **)
 
-instance ilang_is_exportable (#pi:monitorable_prop) (#rcs:tree pck_rc) (#fl:erased tflag) t {| d1: ilang t pi |} : exportable t pi rcs fl = {
+instance ilang_is_exportable (#pi:monitorable_prop) (#rcs:(tree pck_rc){Leaf? rcs}) (#fl:erased tflag) t {| d1: ilang t pi |} : exportable t pi rcs fl = {
   etype = t;
   c_etype = d1;
-  export = (fun eff_rcs x -> x)
+  export = (fun Leaf x -> x)
 }
 
 instance exportable_refinement (#pi:monitorable_prop) (#rcs:tree pck_rc) (#fl:erased tflag) t {| d:exportable t pi rcs fl |} (p : t -> Type0) : exportable (x:t{p x}) pi rcs fl = {
@@ -135,7 +135,7 @@ let lemma_trivialize_new_post_monitorable
   squash (forall x h lt r. (trivialize_new_post_resexn pre post) x h r lt ==> enforced_locally pi h lt) = 
   ()
 
-let trivialize
+let enforce_pre
   #t1 #t2
   (#fl:erased tflag)
   (pre : t1 -> trace -> Type0)
@@ -176,7 +176,7 @@ instance exportable_arrow_with_pre_post
       let (| pck_rc, eff_rc |) = root eff_rcs in
       let rc = Mkdtuple3?._3 pck_rc in
       let eff_rc : eff_rc_typ fl t1 unit (Mkdtuple3?._3 pck_rc) = fast_convert t1 unit _ eff_rc in
-      let f' = trivialize pre rc eff_rc post f in
+      let f' = enforce_pre pre rc eff_rc post f in
       let rc_pre = (fun x h -> rc x h () []) in
       let new_post = trivialize_new_post_resexn rc_pre post in
       let rcs' = (EmptyNode (left rcs) (right rcs)) in
@@ -187,176 +187,165 @@ instance exportable_arrow_with_pre_post
 
     
 (** *** Safe importable instances **)
-let mk_safe_importable
-  (t1 #t2 : Type) {| d1:ilang t1 'pi |}
-  (imp : t1 -> t2) :
-  Tot (safe_importable t2 'pi) =
-  { sitype = t1; c_sitype = d1; safe_import = imp; }
-
-let ilang_is_safely_importable #t (_:ilang t 'pi) : safe_importable t 'pi =
-  mk_safe_importable t (fun x -> x)
+let ilang_is_safely_importable (#pi:monitorable_prop) (#rcs:(tree pck_rc){Leaf? rcs}) (#fl:erased tflag) #t (d:ilang t pi) : safe_importable t pi rcs fl = {
+  sitype = t;
+  c_sitype = d;
+  safe_import = (fun x Leaf -> x); 
+}
 
 (** *** Importable instances **)
 
-let mk_importable
-  (t1 #t2 : Type) {| d1: ilang t1 'pi |}
-  (imp : t1 -> resexn t2) :
-  Tot (importable t2 'pi) =
-  { itype = t1; import = imp; c_itype = d1 }
-
-instance safe_importable_is_importable t {| d:safe_importable t 'pi |} : importable t 'pi =
-  mk_importable d.sitype #t #d.c_sitype
-    (fun (x:d.sitype) -> Inl (safe_import x))
+instance safe_importable_is_importable (#pi:monitorable_prop) (#rcs:tree pck_rc) (#fl:erased tflag) t {| d:safe_importable t pi rcs fl |} : importable t pi rcs fl = {
+  itype = d.sitype;
+  c_itype = d.c_sitype;
+  import = (fun x eff_rcs -> Inl (d.safe_import x eff_rcs))
+}
 
 instance importable_refinement
-  t {| d:importable t 'pi |}
+  (#pi:monitorable_prop) (#rcs:tree pck_rc) (#fl:erased tflag)
+  t {| d:importable t pi rcs fl |}
   (rp : t -> Type0) {| checkable rp |} :
-  Tot (importable (x:t{rp x}) 'pi) =
-  mk_importable
-    d.itype
-    #_
-    #d.c_itype
-    (fun (x:d.itype) ->
-      (match import x with
-      | Inl x ->
-        if check #t #rp x then Inl x 
-        else Inr Contract_failure
-      | Inr err -> Inr err) <: resexn (x:t{rp x}))
-
+  Tot (importable (x:t{rp x}) pi rcs fl) = {
+  itype = d.itype;
+  c_itype = d.c_itype;
+  import = (fun (x:d.itype) eff_rcs ->
+    (match d.import x eff_rcs with
+    | Inl x ->
+      if check #t #rp x then Inl x 
+      else Inr Contract_failure
+    | Inr err -> Inr err) <: resexn (x:t{rp x}))
+}
+    
 instance importable_option
-  t {| d:importable t 'pi |} :
-  Tot (importable (option t) 'pi) =
-  mk_importable
-    (option d.itype)
-    #_
-    #(ilang_option 'pi d.itype #d.c_itype)
-    (fun (x:option d.itype) ->
-      match x with
-      | Some x' -> begin
-        match import x' with
-        | Inl x'' -> Inl (Some x'')
-        | Inr err -> Inr err
-      end
-      | None -> Inr Contract_failure)
+  (#pi:monitorable_prop) (#rcs:tree pck_rc) (#fl:erased tflag)
+  t {| d:importable t pi rcs fl |} :
+  Tot (importable (option t) pi rcs fl) = {
+  itype = option d.itype;
+  c_itype = ilang_option pi d.itype #d.c_itype;
+  import = (fun (x:option d.itype) eff_rcs ->
+    match x with
+    | Some x' -> begin
+      match d.import x' eff_rcs with
+      | Inl x'' -> Inl (Some x'')
+      | Inr err -> Inr err
+    end
+    | None -> Inr Contract_failure)
+}
 
 instance importable_pair
-  t1 t2 {| d1:importable t1 'pi |} {| d2:importable t2 'pi |} :
-  Tot (importable (t1 * t2) 'pi) =
-  mk_importable
-    (d1.itype * d2.itype)
-    #_
-    #(ilang_pair 'pi d1.itype #d1.c_itype d2.itype #d2.c_itype)
-    (fun (x,y) ->
-      match (import x, import y) with
+  (#pi:monitorable_prop) (#rcs:(tree pck_rc){EmptyNode? rcs}) (#fl:erased tflag)
+  t1 t2 {| d1:importable t1 pi (eleft rcs) fl |} {| d2:importable t2 pi (eright rcs) fl |} :
+  Tot (importable (t1 * t2) pi rcs fl) = {
+  itype = d1.itype * d2.itype;
+  c_itype = ilang_pair pi d1.itype #d1.c_itype d2.itype #d2.c_itype;
+  import = (fun (x,y) eff_rcs ->
+      match (d1.import x (eleft eff_rcs), d2.import y (eright eff_rcs)) with
       | (Inl x, Inl y) -> Inl (x, y)
       | _ -> Inr Contract_failure)
+}
 
 instance importable_either
-  t1 t2 {| d1:importable t1 'pi |} {| d2:importable t2 'pi |} :
-  Tot (importable (either t1 t2) 'pi) =
-  mk_importable
-    (either d1.itype d2.itype)
-    #_
-    #(ilang_either 'pi d1.itype #d1.c_itype d2.itype #d2.c_itype)
-    (fun x ->
+  (#pi:monitorable_prop) (#rcs:(tree pck_rc){EmptyNode? rcs}) (#fl:erased tflag)
+  t1 t2 {| d1:importable t1 pi (eleft rcs) fl |} {| d2:importable t2 pi (eright rcs) fl |} :
+  Tot (importable (either t1 t2) pi rcs fl) = {
+  itype = either d1.itype d2.itype;
+  c_itype = ilang_either pi d1.itype #d1.c_itype d2.itype #d2.c_itype;
+  import = (fun x eff_rcs ->
       match x with
       | Inl x' -> begin
-        match import x' with
+        match d1.import x' (eleft eff_rcs) with
         | Inl x'' -> Inl (Inl x'')
         | Inr err -> Inr err
       end
       | Inr y -> begin
-        match import y with
+        match d2.import y (eright eff_rcs) with
         | Inl y' -> Inl (Inr y')
         | Inr err -> Inr err
       end)
+}
 
 instance importable_dpair_refined
+  (#pi:monitorable_prop) (#rcs:(tree pck_rc){EmptyNode? rcs}) (#fl:erased tflag)
   t1 t2 (p:t1 -> t2 -> Type0)
-  {| d1:importable t1 'pi |} {| d2:importable t2 'pi |} {| d3:checkable2 p |} :
-  Tot (importable (x:t1 & y:t2{p x y}) 'pi) =
-  mk_importable
-    (d1.itype & d2.itype)
-    #(x:t1 & y:t2{p x y})
-    #(ilang_pair 'pi d1.itype #d1.c_itype d2.itype #d2.c_itype)
-    (fun ((x', y')) ->
-      match (import x', import y') with
+  {| d1:importable t1 pi (eleft rcs) fl |} {| d2:importable t2 pi (eright rcs) fl |}
+  {| d3:checkable2 p |} :
+  Tot (importable (x:t1 & y:t2{p x y}) pi rcs fl) = {
+  itype = d1.itype & d2.itype;
+  c_itype = ilang_pair pi d1.itype #d1.c_itype d2.itype #d2.c_itype;
+  import = (fun ((x', y')) eff_rcs ->
+      match (d1.import x' (eleft eff_rcs), d2.import y' (eright eff_rcs)) with
        | (Inl x, Inl y) ->
-            if check2 #t1 #t2 #p x y then Inl (| x, y |) else Inr Contract_failure
-       | _ -> Inr Contract_failure) 
-
+            if check2 #t1 #t2 #p x y then Inl ((| x, y |) <: (x:t1 & y:t2{p x y})) else Inr Contract_failure
+       | _ -> Inr Contract_failure)
+}
 
 (** *** Safe importable arrows **)
 instance safe_importable_resexn
-  t1 {| d1:importable t1 'pi |} :
-  Tot (safe_importable (resexn t1) 'pi) =
-  mk_safe_importable
-    (resexn d1.itype)
-    #_
-    #(ilang_resexn 'pi d1.itype #d1.c_itype)
-    (fun x ->
+  (#pi:monitorable_prop) (#rcs:tree pck_rc) (#fl:erased tflag)
+  t1 {| d1:importable t1 pi rcs fl |} :
+  Tot (safe_importable (resexn t1) pi rcs fl) = {
+  sitype = resexn d1.itype;
+  c_sitype = ilang_resexn pi d1.itype #d1.c_itype;
+  safe_import = (fun x eff_rcs ->
       match x with
-      | Inl x' -> import x' 
+      | Inl x' -> d1.import x' eff_rcs 
       | Inr y -> Inr y)
-
+}
+    
 instance safe_importable_arrow
-  (t1:Type) {| d1:exportable t1 'pi |}
-  (t2:Type) {| d2:importable t2 'pi |} : 
-  safe_importable ((x:t1) -> IIOpi (resexn t2) 'pi) 'pi =
-  mk_safe_importable
-    (d1.etype -> IIOpi (resexn d2.itype) 'pi)
-    #((x:t1) -> IIOpi (resexn t2) 'pi)
-    #(ilang_arrow 'pi d1.c_etype (ilang_resexn 'pi d2.itype #d2.c_itype))
-    (fun f (x:t1) -> 
-      (let x' = export x in 
-      safe_import #_ #'pi #(safe_importable_resexn t2 #d2) (f x')))
+  (#pi:monitorable_prop) (#rcs:(tree pck_rc){EmptyNode? rcs}) (#fl:erased tflag)
+  (t1:Type) {| d1:exportable t1 pi (eleft rcs) fl |}
+  (t2:Type) {| d2:importable t2 pi (eright rcs) fl |} : 
+  safe_importable ((x:t1) -> IIOpi (resexn t2) fl pi) pi rcs fl = {
+  sitype = d1.etype -> IIOpi (resexn d2.itype) fl pi;
+  c_sitype = ilang_arrow pi d1.c_etype (ilang_resexn pi d2.itype #d2.c_itype);
+  safe_import = (fun (f:d1.etype -> IIOpi (resexn d2.itype) fl pi) eff_rcs (x:t1) -> 
+    (let x' = d1.export (eleft eff_rcs) x in 
+     let y : resexn d2.itype = f x' in
+     (safe_importable_resexn t2 #d2).safe_import y (eright eff_rcs)) <: IIOpi (resexn t2) fl pi)
+}
 
-let extract_local_trace (h':trace) (pi:monitorable_prop) :
-  IIO trace
-    (requires (fun h -> h' `suffix_of` h))
-    (ensures (fun h lt' lt ->
-      lt == [] /\
-      enforced_locally pi h lt /\
-      h == (apply_changes h' lt'))) =
-  let h = get_trace () in
-  suffix_of_length h' h;
-  let n : nat = (List.length h) - (List.length h') in
-  let (lt', ht) = List.Tot.Base.splitAt n h in
-  lemma_splitAt_equal n h;
-  lemma_splitAt_suffix h h';
-  List.Tot.Properties.rev_involutive lt';
-  assert (h == apply_changes h' (List.rev lt'));
-  List.rev lt'
-
+#set-options "--split_queries"
 let enforce_post
   (#t1 #t2:Type)
+  (#fl:erased tflag)
   (pi:monitorable_prop)
   (pre:t1 -> trace -> Type0)
-  (post:t1 -> trace -> (r:resexn t2) -> trace -> Type0)
-  {| post_c:checkable_hist_post #t1 #t2 pre post pi |}
-  (f:t1 -> IIOpi (resexn t2) pi)
+  (post:t1 -> trace -> (r:resexn t2) -> trace -> (b:Type0{r == Inr Contract_failure ==> b}))
+  (rc : t1 -> trace -> resexn t2 -> trace -> bool)
+  (eff_rc : eff_rc_typ fl t1 (resexn t2) rc) 
+  (c1post : squash (forall x h lt. pre x h /\ enforced_locally pi h lt ==> (exists r. post x h r lt)))
+  (c2post : squash (forall x h r lt. pre x h /\ (rc x h r lt) ==> post x h r lt))
+  (f:t1 -> IIOpi (resexn t2) fl pi)
   (x:t1) :
-  IIO (resexn t2) (pre x) (post x) =
-  let h = get_trace () in
-  let r : resexn t2 = f x in
+  IIO (resexn t2) fl (pre x) (post x) =
+  let (| h, eff_rc' |) = eff_rc x in
   Classical.forall_intro (lemma_suffixOf_append h);
-  let lt = extract_local_trace h pi in
+  let r : resexn t2 = f x in
+  let (lt, b) = eff_rc' r in
   Classical.forall_intro_2 (Classical.move_requires_2 (lemma_append_rev_inv_tail h));
-  if post_c.result_check x h r lt then r
-  else Inr Contract_failure
+  if b then r
+  else (assert (post x h (Inr Contract_failure) lt); Inr Contract_failure)
 
 instance safe_importable_arrow_pre_post
-  (t1:Type) {| d1:exportable t1 'pi |}
-  (t2:Type) {| d2:importable t2 'pi |}
+  (t1:Type) (t2:Type)
+  (#pi:monitorable_prop) 
+  (#rcs:(tree pck_rc){Node? rcs /\ (Mkdtuple3?._1 (root rcs) == t1 /\ (Mkdtuple3?._2 (root rcs) == (resexn t2))) })
+  (#fl:erased tflag)
+  {| d1:exportable t1 pi (left rcs) fl |}
+  {| d2:importable t2 pi (right rcs) fl |}
   (pre : t1 -> trace -> Type0)
   (** it must be `resexn t2` because needs the ability to fail **)
-  (post : t1 -> trace -> (r:resexn t2) -> trace -> Type0)
-  {| post_c:checkable_hist_post #t1 #t2 pre post 'pi |} : 
-  safe_importable ((x:t1) -> IIO (resexn t2) (pre x) (post x)) 'pi =
-  mk_safe_importable
-    (d1.etype -> IIOpi (resexn d2.itype) 'pi)
-    #((x:t1) -> IIO (resexn t2) (pre x) (post x))
-    #(ilang_arrow 'pi d1.c_etype (ilang_resexn 'pi d2.itype #d2.c_itype))
-    (fun f -> 
-      let f' = safe_import #_ #'pi #(safe_importable_arrow t1 #d1 t2 #d2) f in
-      enforce_post 'pi pre post #post_c f')
+  (post : t1 -> trace -> (r:resexn t2) -> trace -> (b:Type0{r == Inr Contract_failure ==> b})) 
+  (c1post : squash (forall x h lt. pre x h /\ enforced_locally pi h lt ==> (exists r. post x h r lt)))
+  (c2post: squash (forall x h r lt. pre x h /\ ((Mkdtuple3?._3 (root rcs)) x h r lt) ==> post x h r lt)) :
+  safe_importable ((x:t1) -> IIO (resexn t2) fl (pre x) (post x)) pi rcs fl = {
+  sitype = d1.etype -> IIOpi (resexn d2.itype) fl pi;
+  c_sitype = ilang_arrow pi d1.c_etype (ilang_resexn pi d2.itype #d2.c_itype);
+  safe_import = (fun (f:(d1.etype -> IIOpi (resexn d2.itype) fl pi)) eff_rcs ->
+    let rcs' = (EmptyNode (left rcs) (right rcs)) in
+    let eff_rcs' = (EmptyNode (left eff_rcs) (right eff_rcs)) in
+    let f' = (safe_importable_arrow #_ #rcs' t1 #d1 t2 #d2).safe_import f eff_rcs' in
+    let (| rc_pck, eff_rc |) = root eff_rcs in
+    enforce_post pi pre post (Mkdtuple3?._3 rc_pck) (fast_convert t1 (resexn t2) _ eff_rc) c1post c2post f')
+}
